

Solved selected problems of Covariant Physics by Moataz Emam

Franco Zacco

Solution. Exercise 1.1

2. For the oblate spheroidal coordinates system if we fix μ to different values we get a set of concentric spheres as we show below If we fix ν we get the following surfaces Finally if we fix ϕ to different values we get that Now, joining all together we get that

□

Solution. Exercise 1.2

Let us consider a point in the x', y', z' coordinate system as shown below
Then we see that

$$\begin{aligned}x &= x' \\y &= y' + z' \sin \alpha \\z &= z' \cos \alpha\end{aligned}$$

Or

$$\begin{aligned}x' &= x \\y' &= y - z \tan \alpha \\z' &= \frac{z}{\cos \alpha}\end{aligned}$$

□

Solution. Exercise 1.3

1. We know that in spherical coordinates

$$\begin{aligned}x^1 &= r \sin \theta \cos \phi \\x^2 &= r \sin \theta \sin \phi \\x^3 &= r \cos \theta\end{aligned}$$

Then

$$\begin{aligned}dx^1 &= d(r \sin \theta \cos \phi) \\&= dr \sin \theta \cos \phi + r d(\sin \theta) \cos \phi + r \sin \theta d(\cos \phi) \\&= dr \sin \theta \cos \phi + r d\theta \cos \theta \cos \phi - r d\phi \sin \theta \sin \phi\end{aligned}$$

$$\begin{aligned}dx^2 &= d(r \sin \theta \sin \phi) \\&= dr \sin \theta \sin \phi + r d(\sin \theta) \sin \phi + r \sin \theta d(\sin \phi) \\&= dr \sin \theta \sin \phi + r d\theta \cos \theta \sin \phi + r d\phi \sin \theta \cos \phi\end{aligned}$$

$$\begin{aligned}dx^3 &= d(r \cos \theta) \\&= dr \cos \theta + r d(\cos \theta) \\&= dr \cos \theta - r d\theta \sin \theta\end{aligned}$$

Let us compute each component $(dx^i)^2$ separately

$$\begin{aligned}(dx^1)^2 &= (dr \sin \theta \cos \phi + r d\theta \cos \theta \cos \phi - r d\phi \sin \theta \sin \phi)^2 \\&= dr^2 \sin^2 \theta \cos^2 \phi + r^2 d\theta^2 \cos^2 \theta \cos^2 \phi + r^2 d\phi^2 \sin^2 \theta \sin^2 \phi \\&\quad + 2r dr d\theta \sin \theta \cos \theta \cos^2 \phi - 2r dr d\phi \sin^2 \theta \cos \phi \sin \phi \\&\quad - 2r^2 d\theta d\phi \cos \theta \cos \phi \sin \theta \sin \phi\end{aligned}$$

$$\begin{aligned}(dx^2)^2 &= (dr \sin \theta \sin \phi + r d\theta \cos \theta \sin \phi + r d\phi \sin \theta \cos \phi)^2 \\&= dr^2 \sin^2 \theta \sin^2 \phi + r^2 d\theta^2 \cos^2 \theta \sin^2 \phi + r^2 d\phi^2 \sin^2 \theta \cos^2 \phi \\&\quad + 2r dr d\theta \sin \theta \cos \theta \sin^2 \phi + r^2 d\theta d\phi \cos \theta \sin \phi \sin \theta \cos \phi \\&\quad + r dr d\phi \sin^2 \theta \sin \phi \cos \phi\end{aligned}$$

$$\begin{aligned}(dx^3)^2 &= (dr \cos \theta - r d\theta \sin \theta)^2 \\&= dr^2 \cos^2 \theta + r^2 d\theta^2 \sin^2 \theta - 2r dr d\theta \cos \theta \sin \theta\end{aligned}$$

Now we sum all components

$$dl^2 = (dx^1)^2 + (dx^2)^2 + (dx^3)^2 = dr^2 + r^2 d\theta^2 + r^2 \sin^2 \theta d\phi^2$$

Where we see that all terms with two different differentials cancel out.

2. We know that the spherical coordinates relate to the cylindrical coordinates as follows

$$\begin{aligned}\rho &= r \sin \theta \\ z &= r \cos \theta \\ \phi &= \phi\end{aligned}$$

Then

$$\begin{aligned}d\rho &= dr \sin \theta + r d\theta \cos \theta \\ dz &= dr \cos \theta - r d\theta \sin \theta \\ d\phi &= d\phi\end{aligned}$$

Also, we know that the line element in cylindrical coordinates is given by

$$dl^2 = d\rho^2 + \rho^2 d\phi^2 + dz^2$$

Hence replacing we get that

$$\begin{aligned}dl^2 &= (dr \sin \theta + r d\theta \cos \theta)^2 + r^2 \sin^2 \theta d\phi^2 + (dr \cos \theta - r d\theta \sin \theta)^2 \\ &= dr^2 \sin^2 \theta + r^2 d\theta^2 \cos^2 \theta + 2r dr d\theta \sin \theta \cos \theta \\ &\quad + r^2 \sin^2 \theta d\phi^2 + dr^2 \cos^2 \theta + r^2 d\theta^2 \sin^2 \theta - 2r dr d\theta \cos \theta \sin \theta \\ &= dr^2 + r^2 d\theta^2 + r^2 \sin^2 \theta d\phi^2\end{aligned}$$

5. We know that in the skew coordinate system we have

$$\begin{aligned}x &= x' \\ y &= y' + z' \sin \alpha \\ z &= z' \cos \alpha\end{aligned}$$

Then

$$\begin{aligned}dx &= dx' \\ dy &= dy' + dz' \sin \alpha \\ dz &= dz' \cos \alpha\end{aligned}$$

Hence the line element in the skew coordinate system is

$$\begin{aligned}dl^2 &= dx^2 + dy^2 + dz^2 \\ &= dx'^2 + (dy' + dz' \sin \alpha)^2 + \cos^2 \alpha dz'^2 \\ &= dx'^2 + dy'^2 + \sin^2 \alpha dz'^2 + 2dy' dz' \sin \alpha + \cos^2 \alpha dz'^2 \\ &= dx'^2 + dy'^2 + dz'^2 + 2dy' dz' \sin \alpha\end{aligned}$$

We see that the metric is not diagonal as expected.

□

Solution. Exercise 1.4

3. The Oblate spheroidal coordinates are defined by

$$x = a \cosh \mu \cos \nu \cos \varphi$$

$$y = a \cosh \mu \cos \nu \sin \varphi$$

$$z = a \sinh \mu \sin \nu$$

Then the scale factors are

$$\begin{aligned} h_\mu^2 &= a^2 \sinh^2 \mu \cos^2 \nu \cos^2 \varphi + a^2 \sinh^2 \mu \cos^2 \nu \sin^2 \varphi + a^2 \cosh^2 \mu \sin^2 \nu \\ &= a^2 \sinh^2 \mu \cos^2 \nu (\cos^2 \varphi + \sin^2 \varphi) + a^2 \cosh^2 \mu \sin^2 \nu \\ &= a^2 \sinh^2 \mu \cos^2 \nu + a^2 \cosh^2 \mu \sin^2 \nu \\ &= a^2 (\sinh^2 \mu \cos^2 \nu + (\sinh^2 \mu + 1) \sin^2 \nu) \\ &= a^2 (\sinh^2 \mu + \sin^2 \nu) \end{aligned}$$

$$\begin{aligned} h_\nu^2 &= a^2 \cosh^2 \mu \sin^2 \nu \cos^2 \varphi + a^2 \cosh^2 \mu \sin^2 \nu \sin^2 \varphi + a^2 \sinh^2 \mu \cos^2 \nu \\ &= a^2 \cosh^2 \mu \sin^2 \nu + a^2 \sinh^2 \mu \cos^2 \nu \\ &= a^2 (\sinh^2 \mu + \sin^2 \nu) \end{aligned}$$

$$\begin{aligned} h_\varphi^2 &= a^2 \cosh^2 \mu \cos^2 \nu \sin^2 \varphi + a^2 \cosh^2 \mu \cos^2 \nu \cos^2 \varphi + 0 \\ &= a^2 \cosh^2 \mu \cos^2 \nu \end{aligned}$$

Hence the line element is given by

$$\begin{aligned} dl^2 &= a^2 (\sinh^2 \mu + \sin^2 \nu) d\mu^2 + a^2 (\sinh^2 \mu + \sin^2 \nu) d\nu^2 + a^2 \cosh^2 \mu \cos^2 \nu d\varphi^2 \\ &= a^2 (\sinh^2 \mu + \sin^2 \nu) (d\mu^2 + d\nu^2) + a^2 \cosh^2 \mu \cos^2 \nu d\varphi^2 \end{aligned}$$

□

Solution. Exercise 1.6

Equation (1.57) states that

$$dl^2 = \delta_{ij} dx^i dx^j$$

If we expand it we get that

$$\begin{aligned} dl^2 &= \delta_{11} dx^1 dx^1 + \delta_{12} dx^1 dx^2 + \delta_{13} dx^1 dx^3 + \delta_{21} dx^2 dx^1 + \delta_{22} dx^2 dx^2 \\ &\quad + \delta_{23} dx^2 dx^3 + \delta_{31} dx^3 dx^1 + \delta_{32} dx^3 dx^2 + \delta_{33} dx^3 dx^3 \\ &= \delta_{11} (dx^1)^2 + \delta_{12} dx^1 dx^2 + \delta_{13} dx^1 dx^3 + \delta_{21} dx^2 dx^1 + \delta_{22} (dx^2)^2 \\ &\quad + \delta_{23} dx^2 dx^3 + \delta_{31} dx^3 dx^1 + \delta_{32} dx^3 dx^2 + \delta_{33} (dx^3)^2 \end{aligned}$$

but we know that $\delta_{ij} = 1$ if $i = j$ and $\delta_{ij} = 0$ if $i \neq j$ then

$$dl^2 = (dx^1)^2 + (dx^2)^2 + (dx^3)^2$$

Which is equation (1.15). □

Solution. Exercise 1.7

1.

$$(\mathbf{A} \cdot \mathbf{B})(\mathbf{C} \cdot \mathbf{D}) = (A^i B^j \delta_{ij})(C^k D^l \delta_{kl}) = (A^i B_i)(C^k D_k)$$

2.

$$\begin{aligned}(\mathbf{A} - \mathbf{B}) \cdot \hat{\mathbf{n}} &= 0 \\ (A^i - B^i) n^j \delta_{ij} &= 0 \\ (A^i - B^i) n_i &= 0\end{aligned}$$

The condition for $\hat{\mathbf{n}}$ to have unit magnitude is $n^i n^j \delta_{ij} = 1$.

3.

$$\cos \theta = \frac{\mathbf{A} \cdot \mathbf{B}}{AB} = \frac{A^i B^j \delta_{ij}}{\sqrt{A^i A^j \delta_{ij}} \sqrt{B^k B^l \delta_{kl}}}$$

4.

$$\mathbf{E} = k \frac{\mathbf{r}}{r^3} = k \frac{x^i \hat{\mathbf{e}}_i}{(\sqrt{x^i x^j \delta_{ij}})^3} = k \frac{x^i \hat{\mathbf{e}}_i}{(x^i x^j \delta_{ij})^{3/2}}$$

5.

$$dW = \mathbf{F} \cdot d\mathbf{r} = F^i dx^j \delta_{ij}$$

6.

$$\frac{1}{2} m v^2 = \frac{1}{2} m (v^i v^j \delta_{ij})$$

□

Solution. Exercise 1.8

1.

$$A_3^1 B_1^2 + A_3^2 B_2^2 + A_3^3 B_3^2 = A_3^i B_i^2$$

2.

$$A_{11}^1 + A_{12}^2 + A_{13}^3 = A_{1i}^i$$

3. The three expressions

$$A^{11} B_1 + A^{12} B_2 + A^{13} B_3 = C^1$$

$$A^{21} B_1 + A^{22} B_2 + A^{23} B_3 = C^2$$

$$A^{31} B_1 + A^{32} B_2 + A^{33} B_3 = C^3$$

can be reduced to

$$A^{ji} B_i = C^j$$

□

Solution. Exercise 1.9

1. Assuming each vector has 3 components we get that

$$\begin{aligned} A_i^j B_j C^i &= A_1^1 B_1 C^1 + A_2^1 B_1 C^2 + A_3^1 B_1 C^3 \\ &\quad + A_1^2 B_2 C^1 + A_2^2 B_2 C^2 + A_3^2 B_2 C^3 \\ &\quad + A_1^3 B_3 C^1 + A_2^3 B_3 C^2 + A_3^3 B_3 C^3 \end{aligned}$$

2. Assuming each vector has 3 components we get that

$$\begin{aligned} A_i B_k^j C^k D_j^i &= A_1 B_1^1 C^1 D_1^1 + A_2 B_1^1 C^1 D_1^2 + A_3 B_1^1 C^1 D_1^3 \\ &\quad + A_1 B_1^2 C^1 D_2^1 + A_2 B_1^2 C^1 D_2^2 + A_3 B_1^2 C^1 D_2^3 \\ &\quad + A_1 B_1^3 C^1 D_3^1 + A_2 B_1^3 C^1 D_3^2 + A_3 B_1^3 C^1 D_3^3 \\ &\quad + A_1 B_2^1 C^2 D_1^1 + A_2 B_2^1 C^2 D_1^2 + A_3 B_2^1 C^2 D_1^3 \\ &\quad + A_1 B_2^2 C^2 D_2^1 + A_2 B_2^2 C^2 D_2^2 + A_3 B_2^2 C^2 D_2^3 \\ &\quad + A_1 B_2^3 C^2 D_3^1 + A_2 B_2^3 C^2 D_3^2 + A_3 B_2^3 C^2 D_3^3 \\ &\quad + A_1 B_3^1 C^3 D_1^1 + A_2 B_3^1 C^3 D_1^2 + A_3 B_3^1 C^3 D_1^3 \\ &\quad + A_1 B_3^2 C^3 D_2^1 + A_2 B_3^2 C^3 D_2^2 + A_3 B_3^2 C^3 D_2^3 \\ &\quad + A_1 B_3^3 C^3 D_3^1 + A_2 B_3^3 C^3 D_3^2 + A_3 B_3^3 C^3 D_3^3 \end{aligned}$$

□

Solution. Exercise 1.10

1. To fix $\mathbf{B} \cdot \mathbf{C} = B^i C_j$ we need to replace the index j by i because of the definition we have in index notation for the dot product i.e. should be $\mathbf{B} \cdot \mathbf{C} = B^i C_i$.
2. In the case of $A^{ij} = B^{ik} C_k^?$ since on the LHS we have two free indexes then on the RHS we should have the same then must be that

$$A^{ij} = B^{ik} C_k^j$$

3. The expression $N_i = R_i^k D_k^p C_?$ is fixed putting p where the question mark is i.e.

$$N_i = R_i^k D_k^p C_p$$

Since the only free index in the LHS is i .

4. The expression $L_k^i D^k = R_m^n N_n^? P^?$ is fixed as follows

$$L_k^i D^k = R_m^n N_n^i P^m$$

or as

$$L_k^i D^k = R_m^n N_n^m P^i$$

Since the only free index in the LHS is i .

5. The expression $\delta^{ij} A_j B_i^k = A^? B_i^k = C^?$ is fixed as follows

$$\delta^{ij} A_j B_i^k = A^i B_i^k = C^k$$

Since we are raising the index in the first equality and we are leaving only k as a free index in the last equality.

6. The expression $N_i = R_i^k \delta_k^p C_? = R_?^? C^?$ is fixed as follows

$$N_i = R_i^k \delta_k^p C_p = R_i^k C^k$$

Since we are raising the index of $C_?$ in the last equality.

□

***Solution.* Exercise 1.12**

1.

$$\mathbf{A} \cdot (\vec{\nabla} f) = A^i \partial_i f$$

2.

$$\vec{\nabla} \cdot \vec{\nabla} f = \partial^i \partial_i f$$

3.

$$\mathbf{A}(\vec{\nabla} \cdot \mathbf{B}) = A^i \partial_j B^j \hat{\mathbf{e}}_i$$

4.

$$\nabla^2 f - \frac{1}{v^2} \frac{\partial^2 f}{\partial t^2} = \partial_i \partial^i f - \frac{1}{v^2} \partial_t^2 f = 0$$

□

Solution. Exercise 1.13

1. Using the product rule we see that

$$\begin{aligned}\partial_k(a_{ij}A^iA^j) &= a_{ij}\partial_k(A^iA^j) \\ &= a_{ij}(A^j(\partial_kA^i) + A^i(\partial_kA^j)) \\ &= 2a_{ij}A^i(\partial_kA^j)\end{aligned}$$

In the third steps we changed the indices because the summation isn't altered by swapping the indices.

2. We know that the notation ∂_ix_j implies $\partial_ix_j = \partial x_j/\partial x_i$ so if $j = i$ then $\partial x_j/\partial x_i = 1$ and if $j \neq i$ we get that $\partial x_j/\partial x_i = 0$ so we can write that $\partial_ix_j = \delta_{ij}$.

In the case of ∂_ix^j we must note first that $x^j = \delta^{kj}x_k$ then

$$\partial_ix^j = \partial_i\delta^{kj}x_k = \delta^{kj}\partial_ix_k = \delta^{kj}\delta_{ik} = \delta_i^j$$

Therefore if $i = j$ then $\partial_ix^j = 1$ and if $i \neq j$ we get that $\partial_ix^j = 0$.

3. We see that

$$\nabla \cdot \mathbf{r} = \partial_ix^i = \frac{\partial x}{\partial x} + \frac{\partial y}{\partial y} + \frac{\partial z}{\partial z} = 3$$

4. Using that $|\mathbf{r}| = \sqrt{x_ix^i}$, the chain rule and the product rule we see that

$$\begin{aligned}\nabla(\ln |\mathbf{r}|) &= \partial^j(\ln \sqrt{x_ix^i})\hat{e}_j \\ &= \frac{1}{2}\partial^j(\ln(x_ix^i))\hat{e}_j \\ &= \frac{1}{2}\left(\frac{\partial^j x_ix^i}{x_kx^k}\right)\hat{e}_j \\ &= \frac{1}{2}\left(\frac{x^i\partial^j x_i + x_i\partial^j x^i}{x_kx^k}\right)\hat{e}_j \\ &= \frac{1}{2}\left(\frac{x^i\delta_i^j + x_i\delta^{ji}}{x_kx^k}\right)\hat{e}_j \\ &= \frac{1}{2}\left(\frac{x^j + x^j}{x_kx^k}\right)\hat{e}_j \\ &= \frac{x^j\hat{e}_j}{x_kx^k} \\ &= \frac{\mathbf{r}}{r^2}\end{aligned}$$

5. Let us note that $\nabla^2 = \nabla \cdot \nabla$, so reusing the result from part 4 we see that

$$\begin{aligned}
\nabla^2(\ln |\mathbf{r}|) &= \nabla \cdot \nabla(\ln |\mathbf{r}|) \\
&= \partial_j \frac{x^j}{x_k x^k} \\
&= x^j \partial_j \frac{1}{x_k x^k} + \frac{1}{x_k x^k} \partial_j x^j \\
&= -x^j \frac{\partial_j x_k x^k}{(x_k x^k)^2} + \frac{3}{x_k x^k} \\
&= -x^j \frac{x^k \partial_j x_k + x_k \partial_j x^k}{(x_k x^k)^2} + \frac{3}{x_k x^k} \\
&= -x^j \frac{x^k \delta_{jk} + x_k \delta_j^k}{(x_k x^k)^2} + \frac{3}{x_k x^k} \\
&= -\frac{2x_j x^j}{(x_k x^k)^2} + \frac{3}{x_k x^k} \\
&= -\frac{2r^2}{(r^2)^2} + \frac{3}{r^2} \\
&= -\frac{2}{r^2} + \frac{3}{r^2} \\
&= \frac{1}{r^2}
\end{aligned}$$

Where we used that $\partial_j x^j = 3$ from part 3.

□

Solution. Exercise 1.14

1. Equation 1.99 states that

$$\mathbf{C} = \delta^{ni} \varepsilon_{ijk} A^j B^k \hat{\mathbf{e}}_n$$

Expanding the equation we get that

$$\begin{aligned} \mathbf{C} &= \delta^{11} \varepsilon_{123} A^2 B^3 \hat{\mathbf{e}}_1 + \delta^{11} \varepsilon_{132} A^3 B^2 \hat{\mathbf{e}}_1 + \\ &\quad + \delta^{22} \varepsilon_{213} A^1 B^3 \hat{\mathbf{e}}_2 + \delta^{22} \varepsilon_{231} A^3 B^1 \hat{\mathbf{e}}_2 + \\ &\quad + \delta^{33} \varepsilon_{321} A^2 B^1 \hat{\mathbf{e}}_3 + \delta^{33} \varepsilon_{312} A^1 B^2 \hat{\mathbf{e}}_3 \\ &= \varepsilon_{123} A^2 B^3 \hat{\mathbf{e}}_1 - \varepsilon_{123} A^3 B^2 \hat{\mathbf{e}}_1 - \varepsilon_{231} A^1 B^3 \hat{\mathbf{e}}_2 + \varepsilon_{231} A^3 B^1 \hat{\mathbf{e}}_2 \\ &\quad - \varepsilon_{312} A^2 B^1 \hat{\mathbf{e}}_3 + \varepsilon_{312} A^1 B^2 \hat{\mathbf{e}}_3 \\ &= \varepsilon_{123} (A^2 B^3 - A^3 B^2) \hat{\mathbf{e}}_1 + \varepsilon_{231} (A^3 B^1 - A^1 B^3) \hat{\mathbf{e}}_2 \\ &\quad + \varepsilon_{312} (A^1 B^2 - A^2 B^1) \hat{\mathbf{e}}_3 \\ &= (A^2 B^3 - A^3 B^2) \hat{\mathbf{e}}_1 + (A^3 B^1 - A^1 B^3) \hat{\mathbf{e}}_2 + (A^1 B^2 - A^2 B^1) \hat{\mathbf{e}}_3 \end{aligned}$$

Where we only wrote the non-zero terms and we used the rules of the Levi-Civita symbol.

Equations (1.100) and (1.101) are essentially the same calculations.

3. Equation (1.106) states that

$$\varepsilon_{ijk} \varepsilon^{mnl} = \delta_i^m (\delta_j^n \delta_k^l - \delta_j^l \delta_k^n) - \delta_i^n (\delta_j^m \delta_k^l - \delta_j^l \delta_k^m) + \delta_i^l (\delta_j^m \delta_k^n - \delta_j^n \delta_k^m)$$

Then if $l = k$ we get that

$$\begin{aligned} \varepsilon_{ijk} \varepsilon^{mnk} &= \delta_i^m (\delta_j^n \delta_k^k - \delta_j^k \delta_k^n) - \delta_i^n (\delta_j^m \delta_k^k - \delta_j^k \delta_k^m) + \delta_i^k (\delta_j^m \delta_k^n - \delta_j^n \delta_k^m) \\ &= \delta_i^m (3\delta_j^n - \delta_j^n) - \delta_i^n (3\delta_j^m - \delta_j^m) + \delta_i^k (\delta_j^m \delta_k^n - \delta_j^n \delta_k^m) \\ &= 2\delta_i^m \delta_j^n - 2\delta_i^n \delta_j^m + \delta_i^k \delta_j^m \delta_k^n - \delta_i^k \delta_j^n \delta_k^m \\ &= 2\delta_i^m \delta_j^n - 2\delta_i^n \delta_j^m + \delta_j^m \delta_i^n - \delta_j^n \delta_i^m \\ &= \delta_i^m \delta_j^n - \delta_i^n \delta_j^m \end{aligned}$$

If $n = j$ and $l = k$ we get that

$$\varepsilon_{ijk} \varepsilon^{mjk} = \delta_i^m \delta_j^j - \delta_i^j \delta_j^m = 3\delta_i^m - \delta_i^m = 2\delta_i^m$$

And if $m = i$, $n = j$ and $l = k$

$$\varepsilon_{ijk} \varepsilon^{ijk} = 2\delta_i^i = 2 \cdot 3 = 6$$

4. Our guess for the formula equivalent to (1.106) for the case of the two-dimensional Levi-Civita symbol is

$$\varepsilon_{ij}\varepsilon^{mn} = \delta_i^m \delta_j^n - \delta_i^n \delta_j^m$$

We check this guess by computing the components.

$$\begin{aligned}\varepsilon_{12}\varepsilon^{12} &= 1 = 1 - 0 = \delta_1^1 \delta_2^2 - \delta_1^2 \delta_2^1 \\ \varepsilon_{21}\varepsilon^{12} &= -1 = 0 - 1 = \delta_2^1 \delta_1^2 - \delta_2^2 \delta_1^1 \\ \varepsilon_{12}\varepsilon^{21} &= -1 = 0 - 1 = \delta_1^2 \delta_2^1 - \delta_1^1 \delta_2^2 \\ \varepsilon_{21}\varepsilon^{21} &= 1 = 1 - 0 = \delta_2^2 \delta_1^1 - \delta_2^1 \delta_1^2\end{aligned}$$

For the components where $i = j$ we have that

$$\varepsilon_{ii}\varepsilon^{mn} = 0 = \delta_i^m \delta_i^n - \delta_i^n \delta_i^m$$

And for the components where $m = n$ we get that

$$\varepsilon_{ij}\varepsilon^{mm} = 0 = \delta_i^m \delta_j^m - \delta_i^m \delta_j^m$$

Therefore our guess is correct.

Let us compute the identities similar to (1.107) as follows

$$\begin{aligned}\varepsilon_{ij}\varepsilon^{mj} &= \delta_i^m \delta_j^j - \delta_i^j \delta_j^m = 3\delta_i^m - \delta_i^m = 2\delta_i^m \\ \varepsilon_{ij}\varepsilon^{ij} &= 2\delta_i^i = 6\end{aligned}$$

□

Solution. Exercise 1.15

Let A^{ij} be any matrix then we can write it as

$$A^{ij} = \frac{1}{2}(A^{ij} + A^{ji}) + \frac{1}{2}(A^{ij} - A^{ji})$$

Let us consider the two terms as independent matrices.

If we define $B^{ij} = \frac{1}{2}(A^{ij} + A^{ji})$ we see that

$$B^{ji} = \frac{1}{2}(A^{ji} + A^{ij}) = \frac{1}{2}(A^{ij} + A^{ji}) = B^{ij}$$

So we see that B^{ij} is a totally symmetric matrix.

On the other hand, let us define $C^{ij} = \frac{1}{2}(A^{ij} - A^{ji})$, then we see that

$$C^{ji} = \frac{1}{2}(A^{ji} - A^{ij}) = -\frac{1}{2}(A^{ij} - A^{ji}) = -C^{ij}$$

So C^{ij} is a totally antisymmetric matrix.

Therefore we may write A^{ij} as

$$A^{ij} = A^{(ij)} + A^{[ij]}$$

Where $B^{ij} = A^{(ij)}$ and $C^{ij} = A^{[ij]}$ and hence

$$A^{(ij)} = \frac{1}{2}(A^{ij} + A^{ji}) \quad A^{[ij]} = \frac{1}{2}(A^{ij} - A^{ji})$$

□

Solution. Exercise 1.16

To decompose the matrix

$$A = \begin{bmatrix} 1 & 1 & 2 \\ -3 & 2 & -3 \\ 4 & 3 & 3 \end{bmatrix}$$

We need to compute each element of the totally symmetric matrix A_s and the totally antisymmetric matrix A_a , for this we use the equations (1.113) as follows

$$\begin{aligned} A_s^{(11)} &= \frac{1}{2}(A_s^{11} + A_s^{11}) = \frac{1}{2}(1 + 1) = 1 \\ A_s^{(12)} &= \frac{1}{2}(A_s^{12} + A_s^{21}) = \frac{1}{2}(1 - 3) = -1 \\ A_s^{(13)} &= \frac{1}{2}(A_s^{13} + A_s^{31}) = \frac{1}{2}(2 + 4) = 3 \end{aligned}$$

Given that A_s is totally symmetric we know that $A_s^{(21)} = A_s^{(12)}$ and $A_s^{(31)} = A_s^{(13)}$ hence the only element left to compute is $A_s^{(23)} = A_s^{(32)}$

$$A_s^{(23)} = \frac{1}{2}(A_s^{23} + A_s^{32}) = \frac{1}{2}(-3 + 3) = 0$$

Then the totally symmetric matrix is

$$A_s = \begin{bmatrix} 1 & -1 & 3 \\ -1 & 2 & 0 \\ 3 & 0 & 3 \end{bmatrix}$$

For the totally antisymmetric matrix A_a we compute what follows

$$\begin{aligned} A_a^{[11]} &= \frac{1}{2}(A_a^{11} - A_a^{11}) = \frac{1}{2}(1 - 1) = 0 \\ A_a^{[12]} &= \frac{1}{2}(A_a^{12} - A_a^{21}) = \frac{1}{2}(1 + 3) = 2 \\ A_a^{[13]} &= \frac{1}{2}(A_a^{13} - A_a^{31}) = \frac{1}{2}(2 - 4) = -1 \end{aligned}$$

And computing the element $A_a^{[23]}$ we have all we need to get A_a

$$A_a^{[23]} = \frac{1}{2}(A_a^{23} - A_a^{32}) = \frac{1}{2}(-3 - 3) = -3$$

Then the matrix A_a is

$$A_a = \begin{bmatrix} 0 & 2 & -1 \\ -2 & 0 & -3 \\ 1 & 3 & 0 \end{bmatrix}$$

Finally, we can compute the sum $A_s + A_a$ to check that the matrices are correct, we should get A .

$$A_s + A_a = \begin{bmatrix} 1 & -1 & 3 \\ -1 & 2 & 0 \\ 3 & 0 & 3 \end{bmatrix} + \begin{bmatrix} 0 & 2 & -1 \\ -2 & 0 & -3 \\ 1 & 3 & 0 \end{bmatrix} = \begin{bmatrix} 1 & 1 & 2 \\ -3 & 2 & -3 \\ 4 & 3 & 3 \end{bmatrix} = A$$

□

Solution. Exercise 1.17

1. Let $\varepsilon_{ijk}A^k = B_{ij}$ then multiplying both sides by ε^{ijl} we get that

$$\begin{aligned}\varepsilon_{ijk}\varepsilon^{ijl}A^k &= \varepsilon^{ijl}B_{ij} \\ 2\delta_k^l A^k &= \varepsilon^{ijl}B_{ij} \\ 2A^l &= \varepsilon^{ijl}B_{ij} \\ A^l &= \frac{1}{2}\varepsilon^{ijl}B_{ij}\end{aligned}$$

2. Let now A^{jk} be totally antisymmetric and let also $\varepsilon_{ijk}A^{jk} = B_i$ then

$$\begin{aligned}\varepsilon^{inm}\varepsilon_{ijk}A^{jk} &= \varepsilon^{inm}B_i \\ (\delta_j^n \delta_k^m - \delta_k^n \delta_j^m)A^{jk} &= \varepsilon^{inm}B_i \\ \delta_j^n \delta_k^m A^{jk} - \delta_k^n \delta_j^m A^{jk} &= \varepsilon^{inm}B_i \\ A^{nm} - A^{mn} &= \varepsilon^{inm}B_i\end{aligned}$$

But A is totally antisymmetric so $A^{mn} = -A^{nm}$ and hence

$$\begin{aligned}A^{nm} + A^{nm} &= \varepsilon^{inm}B_i \\ A^{nm} &= \frac{1}{2}\varepsilon^{inm}B_i\end{aligned}$$

3. Let now A^{jk} be totally symmetric and let also $\varepsilon_{ijk}A^{jk} = B_i$ then

$$\begin{aligned}\varepsilon^{inm}\varepsilon_{ijk}A^{jk} &= \varepsilon^{inm}B_i \\ \varepsilon^{nmi}\varepsilon_{jki}A^{jk} &= \varepsilon^{inm}B_i \\ (\delta_j^n \delta_k^m - \delta_j^m \delta_k^n)A^{jk} &= \varepsilon^{inm}B_i \\ \delta_j^n \delta_k^m A^{jk} - \delta_j^m \delta_k^n A^{jk} &= \varepsilon^{inm}B_i \\ A^{nm} - A^{mn} &= \varepsilon^{inm}B_i \\ A^{nm} - A^{nm} &= \varepsilon^{inm}B_i \\ 0 &= B_i\end{aligned}$$

Where we used that A is totally symmetric so $A^{mn} = A^{nm}$, then since $B_i = 0$ we have that $\varepsilon_{ijk}A^{jk} = 0$.

4. If A^{jk} is neither totally symmetric nor totally antisymmetric then we get that

$$A^{nm} - A^{mn} = \varepsilon^{inm}B_i$$

But we can write A^{nm} as the sum of a totally symmetric and a totally antisymmetric matrix so

$$\begin{aligned} A^{(nm)} + A^{[nm]} - A^{(mn)} - A^{[mn]} &= \varepsilon^{inm} B_i \\ A^{(nm)} + A^{[nm]} - A^{(nm)} + A^{[nm]} &= \varepsilon^{inm} B_i \\ 2A^{[nm]} &= \varepsilon^{inm} B_i \\ A^{[nm]} &= \frac{1}{2} \varepsilon^{inm} B_i \end{aligned}$$

So as we saw in part 2 the antisymmetric matrix will be of the form $\frac{1}{2} \varepsilon^{inm} B_i$ but we cannot say anything about the symmetric part.

5. Let $\delta^{ik} \varepsilon_{ijn} A^n = B_j^k$ then

$$\begin{aligned} \delta^{ik} \varepsilon_{ijn} A^n &= B_j^k \\ \varepsilon^k{}_{jn} A^n &= B_j^k \\ \varepsilon_k{}^{jl} \varepsilon^k{}_{jn} A^n &= \varepsilon_k{}^{jl} B_j^k \\ 2\delta_n^l A^n &= \varepsilon_k{}^{jl} B_j^k \\ A^l &= \frac{1}{2} \varepsilon_k{}^{jl} B_j^k \end{aligned}$$

□